Utils/TLAmore.v
@@ -1,0 +1,93 @@
+From TLA Require Export logic.
+
+Section Proof_Env.
+
+  Context [Σ : Type].
+  Variable (Γ Γ' : predicate Σ).
+
+  (* combining two leads_to things *)
+
+  Fact leads_to_combine (p1 q1 p2 q2 : predicate Σ)
+    (* making Γ persistent would be convenient *)
+    (H1 : □ Γ ∧ Γ' ⊢ p1 ~~> q1) (H2 : □ Γ ∧ Γ' ⊢ p2 ~~> q2)
+    (* q1 and q2 have to be persistent *)
+    (* writing H1' and H2' in this way would align with the form of invariant *)
+    (H1' : q1 ∧ □ Γ ⊢ □ q1) (H2' : q2 ∧ □ Γ ⊢ □ q2) : 
+    □ Γ ∧ Γ' ⊢ (p1 ∧ p2) ~~> (q1 ∧ q2).
+  Proof.
+    autounfold with tla in *.
+    intros.
+    destruct H0.
+    specialize (H1 _ H k H0).
+    specialize (H2 _ H k H3).
+    destruct H1 as (k1 & H1), H2 as (k2 & H2).
+    rewrite ! drop_drop in H1, H2.
+    destruct H.
+    assert (∀ (k k0 : nat), Γ (drop k (drop k0 e))) as H' 
+      by (intros; now rewrite drop_drop).
+    specialize (H1' _ (conj H1 (fun k => H' k _)) (Nat.max k1 k2 - k1)).
+    specialize (H2' _ (conj H2 (fun k => H' k _)) (Nat.max k1 k2 - k2)).
+    rewrite ! drop_drop in H1', H2'.
+    replace (drop _ e) with (drop (Nat.max k1 k2 + k) e) in H1' by (f_equal; lia).
+    replace (drop _ e) with (drop (Nat.max k1 k2 + k) e) in H2' by (f_equal; lia).
+    repeat setoid_rewrite drop_drop.
+    eauto.
+  Qed.
+
+  Context [A : Type].
+  Variable (valid : A → Prop) (l : list A).
+  Hypothesis (Hvalid : Forall valid l).  
+
+  Fact leads_to_combine_batch (p q : A → predicate Σ)
+    (H : ∀ a, valid a → (□ Γ ∧ Γ' ⊢ (p a) ~~> (q a))%L)
+    (H' : ∀ a, valid a → ((q a) ∧ □ Γ ⊢ □ (q a))%L) :
+    (□ Γ ∧ Γ' ⊢ (fold_right tla_and tla_true (map p l)) ~~> 
+      (fold_right tla_and tla_true (map q l)))%L ∧
+    (* the following needs to be proved together by induction *)
+    ((fold_right tla_and tla_true (map q l)) ∧ □ Γ ⊢
+      (□ fold_right tla_and tla_true (map q l)))%L.
+  Proof using All.
+    induction Hvalid as [ | a l Hv Hvalid' IH ]; simpl.
+    - split.
+      + now apply impl_drop_hyp, impl_to_leads_to.
+      + now autounfold with tla.
+    - specialize (IH Hvalid').
+      destruct IH as (IH1 & IH2).
+      split.
+      + apply leads_to_combine; auto.
+      + rewrite always_and.
+        tla_split.
+        * now tla_apply H'.
+        * now tla_apply IH2.
+  Qed.
+
+  Corollary leads_to_combine_batch' (p q : A → Σ → Prop)
+    (H : ∀ a, valid a → (□ Γ ∧ Γ' ⊢ ⌜ p a ⌝ ~~> ⌜ q a ⌝)%L)
+    (H' : ∀ a, valid a → (⌜ q a ⌝ ∧ □ Γ ⊢ □ ⌜ q a ⌝)%L) :
+    □ Γ ∧ Γ' ⊢ 
+      ⌜ λ w, (∀ a, In a l → p a w) ⌝ ~~> ⌜ λ w, (∀ a, In a l → q a w) ⌝.
+  Proof using All.
+    tla_pose (proj1 (leads_to_combine_batch _ _ H H')).
+    clear Hvalid.
+    tla_apply leads_to_weaken.
+    all: autounfold with tla; intros.
+    - rewrite <- Forall_forall in H0.
+      induction H0; simpl; auto.
+    - revert a H1.
+      rewrite <- Forall_forall.
+      induction l; simpl in H0; auto.
+      constructor; intuition.
+  Qed.
+
+End Proof_Env.
+
+(* more notations *)
+
+Definition satisfies {Σ : Type} (p : predicate Σ) (e : exec Σ) := p e.
+(* TODO any pure predicate in the formalism of TLA? *)
+Definition pure_pred {Σ : Type} (P : Prop) : predicate Σ := ⌜ λ _, P ⌝.
+
+Notation "e ⊨ p" := (satisfies p%L e) (at level 100).
+Notation "⌞  P  ⌟" := (pure_pred P%type).
+
+#[export] Hint Unfold pure_pred satisfies : tla.
